valuability, seqt, totality, and eta sequal rules

coq/Defs.v
@@ -52,7 +52,6 @@ Definition acc : fterm :=
 Definition admiss : fterm := lam (admiss (var 0)).
 Definition bool : fterm := booltp.
 Definition bottom : fterm := app theta (lam (var 0)).
-Definition coguard : fterm := lam (lam (coguard (var 1) (var 0))).
 Definition eeqtp : fterm := lam (lam (prod (subtype (var 1) (var 0)) (subtype (var 0) (var 1)))).
 Definition eq : fterm := lam (lam (lam (equal (var 2) (var 1) (var 0)))).
 Definition eqtp : fterm := lam (lam (eqtype (var 1) (var 0))).
@@ -64,8 +63,7 @@ Definition iexists : fterm := lam (lam (lam (exist (var 2) (var 1) (app (var 1) 
 Definition iff : fterm := lam (lam (prod (pi (var 1) (var 1)) (pi (var 0) (var 2)))).
 Definition iforall : fterm := lam (lam (lam (all (var 2) (var 1) (app (var 1) (var 0))))).
 Definition intersect : fterm := lam (lam (intersect (var 1) (app (var 1) (var 0)))).
-Definition union : fterm := lam (lam (union (var 1) (app (var 1) (var 0)))).
-Definition halts : fterm := lam (halts (var 0)).
+Definition iset : fterm := lam (lam (iset (var 1) (app (var 1) (var 0)))).
 Definition istp : fterm := lam (eqtype (var 0) (var 0)).
 Definition ite : fterm := lam (lam (lam (bite (var 2) (var 1) (var 0)))).
 Definition karrow : fterm := lam (lam (karrow (var 1) (var 0))).
@@ -90,7 +88,6 @@ Definition mu : fterm := lam (mu (app (var 1) (var 0))).
 Definition nat : fterm := nattp.
 Definition negative : fterm := lam (isnegative (app (var 1) (var 0))).
 Definition of : fterm := lam (lam (equal (var 1) (var 0) (var 0))).
-Definition partial : fterm := lam (partial (var 0)).
 Definition prod : fterm := lam (lam (prod (var 1) (var 0))).
 Definition quotient : fterm := lam (lam (quotient (var 1) (app (app (var 2) (var 1)) (var 0)))).
 Definition rec : fterm := lam (rec (app (var 1) (var 0))).
@@ -98,16 +95,19 @@ Definition positive : fterm := lam (ispositive (app (var 1) (var 0))).
 Definition seq : fterm := lam (lam (seq (var 1) (app (var 1) (var 0)))).
 Definition sequal : fterm := lam (lam (sequal (var 1) (var 0))).
 Definition squash : fterm := lam (set unittp (var 1)).
-Definition subtype : fterm := lam (lam (subtype (var 1) (var 0))).
 Definition succ : fterm := lam (app inr (var 0)).
 Definition sum : fterm := lam (lam (sigma booltp (bite (var 0) (var 2) (var 1)))).
 Definition tarrow : fterm := lam (lam (tarrow (var 1) (var 0))).
 Definition true : fterm := btrue.
+Definition union : fterm := lam (lam (union (var 1) (app (var 1) (var 0)))).
 Definition unit : fterm := unittp.
 Definition univ : fterm := lam (univ (var 0)).
+Definition uptype : fterm := lam (uptype (var 0)).
 Definition void : fterm := voidtp.
+Definition wind : fterm := lam (wind (var 0)).
 Definition wtype : fterm := lam (lam (wt (var 1) (app (var 1) (var 0)))).
 Definition zero : fterm := app inl triv.
+Definition triv : fterm := triv.
 
 Definition sum_case : fterm := 
   lam (lam (lam (bite 
@@ -134,13 +134,18 @@ Definition max : fterm :=
                                        (app succ
                                           (app (app (var 4) (var 1)) (var 0)))))))))).
 
-Definition set : fterm := lam (lam (set (var 1) (app (var 1) (var 0)))).
-Definition iset : fterm := lam (lam (iset (var 1) (app (var 1) (var 0)))).
-Definition sigma : fterm := lam (lam (sigma (var 1) (app (var 1) (var 0)))).
-Definition theta : fterm := theta.
-Definition triv : fterm := triv.
-Definition uptype : fterm := lam (uptype (var 0)).
-Definition wind : fterm := lam (wind (var 0)).
+Definition total : fterm :=
+  lam (sigma
+         (subtype (var 0) (partial (var 0)))
+         (pi (var 1) (halts (var 0)))).
 
 Definition arrow : fterm := lam (lam (pi (var 1) (var 1))).
+Definition coguard : fterm := lam (lam (coguard (var 1) (var 0))).
+Definition halts : fterm := lam (halts (var 0)).
+Definition partial : fterm := lam (partial (var 0)).
+Definition set : fterm := lam (lam (set (var 1) (app (var 1) (var 0)))).
+Definition subtype : fterm := lam (lam (subtype (var 1) (var 0))).
+Definition theta : fterm := theta.
+
 Definition pi : fterm := lam (lam (pi (var 1) (app (var 1) (var 0)))).
+Definition sigma : fterm := lam (lam (sigma (var 1) (app (var 1) (var 0)))).
